Add Dan's suggestions for cleanup

theories/PushoutPath/PushoutPath.v
@@ -51,19 +51,21 @@ Section InductiveStep.
     := fun a b r p => inverse (pglue ((b ; r) , p)).
 End InductiveStep.
 
+Definition Dot {A B : Type} (R : A -> B -> Type) (P : Family A) (Q : Family B)
+  := forall (a : A) (b : B) (r : R a b) (p : P a), Q b.
 Section Sequence.
   Context {A B : Type} (R : A -> B -> Type) (a0 : A).
 
   (** Use a record type for a full step to avoid the interleaved sequence and `flip R`. *)
   Record zigzag_type : Type := {
-    Pp : A -> Type; (** Stored from previous step *)
-    Qp : B -> Type; (** Stored from previous step *)
-    concatQPp (b : B) (a : A) (r : R a b) (q : Qp b) : Pp a; (** Stored from previous step *)
-    Q : B -> Type; (** Paths of length t *)
-    concatPQ (a : A) (b : B) (r : R a b) (p : Pp a) : Q b; (** t-1 -> t *)
+    Pp : Family A; (** Stored from previous step *)
+    Qp : Family B; (** Stored from previous step *)
+    concatQPp : Dot (flip R) Qp Pp; (** Stored from previous step *)
+    Q : Family B; (** Paths of length t *)
+    concatPQ : Dot R Pp Q; (** t-1 -> t *)
     iotaQ (b : B) (x : Qp b) : Q b; (** t-2 -> t *)
-    P : A -> Type; (** Paths of length t+1 *)
-    concatQP (b : B) (a : A) (r : R a b) (q : Q b) : P a; (** t -> t+1 *)
+    P : Family A; (** Paths of length t+1 *)
+    concatQP : Dot (flip R) Q P; (** t -> t+1 *)
     iotaP (a : A) (x : Pp a) : P a; (** t-1 -> t+1 *)
     concatQPQ (b : B) (a : A) (r : R a b) 
       : (compose (concatPQ a b r) (concatQPp b a r)) == (iotaQ b);
@@ -73,21 +75,18 @@ Section Sequence.
 
   Definition zigzag_step : zigzag_type -> zigzag_type.
   Proof.
-    intro z.
-    destruct z.
+    intros [_ _ _ Q0 _ _ P0 concatQP0 _ _ _];
+    pose (concatPQ := dot_step (flip R) concatQP0).
     (* Naming them all seems to be necessary for Coq to not reorder goals. *)
-    snrapply (let Pp:=_ in let Qp :=_ in let concatQPp :=_ in let Q:=_ in let concatPQ:=_ in let iotaQ:=_ in let P:=_ in let concatQP:=_ in let iotaP:=_ in let concatQPQ:=_ in let concatPQP:=_ in Build_zigzag_type Pp Qp concatQPp Q concatPQ iotaQ P concatQP iotaP concatQPQ concatPQP).
-    - exact P0.
-    - exact Q0.
-    - exact concatQP0.
-    - exact (family_step (flip R) concatQP0).
-    - exact (dot_step (flip R) concatQP0).
-    - exact (iota_step (flip R) concatQP0).
-    - exact (family_step R concatPQ).
-    - exact (dot_step R concatPQ).
-    - exact (iota_step R concatPQ).
-    - exact (homotopy_step (flip R) concatQP0).
-    - exact (homotopy_step R concatPQ).
+    snrapply (Build_zigzag_type P0 Q0 concatQP0).
+      - exact (family_step (flip R) concatQP0).
+      - exact concatPQ.
+      - exact (iota_step (flip R) concatQP0).
+      - exact (family_step R concatPQ).
+      - exact (dot_step R concatPQ).
+      - exact (iota_step R concatPQ).
+      - exact (homotopy_step (flip R) concatQP0).
+      - exact (homotopy_step R concatPQ).
   Defined.
 
   Definition identity_zigzag_initial : zigzag_type.
